Technique/TechniqueOneStep.v
@@ -1,12 +1,13 @@
 Require Import Coq.Lists.List.
 
 Require Import Machine.Machine.
+Require Import Machine.MachineValid.
 Require Import Attacker.Attacker.
 Require Import Technique.Technique.
 Require Import Technique.TechniquePreCondition.
 Require Import Technique.TechniquePostCondition.
 
-Inductive one_step : Attacker -> Technique -> (idMachine -> option Machine) -> Attacker -> Prop :=
-      | onestep : forall (a: Attacker) (t: Technique) (network: idMachine -> option Machine) (a': Attacker),
-                    valid_network network -> valid_attacker a network -> Pre a t -> Post a t network a' -> one_step a t network a'.
+Inductive one_step : Attacker -> Technique -> (network_map) -> Attacker -> Prop :=
+      | onestep : forall (a: Attacker) (t: Technique) (network: network_map) (a': Attacker),
+                    valid_concrete_network network -> valid_attacker a network -> Pre a t -> Post a t network a' -> one_step a t network a'.
                     
