Invariant/ValidAttacker/ValidAttacker.v
@@ -1,0 +1,25 @@
+Require Import Machine.Machine.
+Require Import Machine.MachineValid.
+Require Import Machine.MachineAuxFunctions.
+Require Import Attacker.Attacker.
+Require Import Technique.Technique.
+Require Import Technique.TechniquePreCondition.
+Require Import Technique.TechniquePostCondition.
+Require Import Technique.TechniqueOneStep.
+
+Require Import Invariant.ValidAttacker.ValidAttackerI.OneStepPreservesValidAttackerI.
+Require Import Invariant.ValidAttacker.ValidAttackerII.OneStepPreservesValidAttackerII.
+Require Import Invariant.ValidAttacker.ValidAttackerIII.OneStepPreservesValidAttackerIII.
+Require Import Invariant.ValidAttacker.ValidAttackerIV.OneStepPreservesValidAttackerIV.
+
+Theorem one_step_preserves_valid_attacker : forall (a a' : Attacker) (t : Technique) (n: network_map),
+      one_step a t n a' -> valid_attacker a' n.
+  Proof.
+    intros a a' t n onestep.
+    unfold valid_attacker.
+    split; [  | split]; [ | | split].
+    - apply (one_step_preserves_valid_attacker_i a a' t n); auto.
+    - apply (one_step_preserves_valid_attacker_ii a a' t n); auto.
+    - apply (one_step_preserves_valid_attacker_iii a a' t n); auto.
+    - apply (one_step_preserves_valid_attacker_iv a a' t n); auto.
+  Qed.
