Invariant/ValidAttacker/ValidAttackerI/RemoteServices.v
@@ -1,18 +1,18 @@
 Require Import Coq.Lists.List.
 
 Require Import Machine.Machine.
+Require Import Machine.MachineValid.
 Require Import Machine.MachineAuxFunctions.
 Require Import Attacker.Attacker.
 Require Import Technique.Technique.
 Require Import Technique.TechniquePreCondition.
 Require Import Technique.TechniquePostCondition.
-Require Import Technique.TechniqueOneStep.
 
 Require Import Invariant.AuxLemmas.AuxLemmas.
 Require Import Invariant.AuxTactics.
 
 Lemma one_step_remote_services_preserves_valid_attacker_i : forall (a a' : Attacker) (n: network_map) (aValid: valid_attacker a n) (m m': idMachine) (u u': idUser) (k': key) (s': idService),
-      valid_network n -> Pre a (Remote_Services m u m' u' k' s') -> Post a (Remote_Services m u m' u' k' s') n a' -> valid_attacker_i a' n.
+      valid_network n -> Pre a (Remote_Services m u m' u' k' s') -> Post a (Remote_Services m u m' u' k' s') n a' -> valid_attacker_i a'.
   Proof.
     intros a a' network validAttacker m m' u u' k' s' validNetwork pre post.
     unfold valid_attacker_i.
