Invariant/ValidAttacker/ValidAttackerII/OneStepPreservesValidAttackerII.v
@@ -12,15 +12,12 @@ Require Import Technique.TechniqueOneStep.
 Require Import Invariant.AuxLemmas.AuxLemmas.
 Require Import Invariant.AuxTactics.
 
-Require Import Invariant.ValidAttacker.ValidAttackerI.RemoteServices.
-
-Theorem one_step_preserves_valid_attacker_i : forall (a a' : Attacker) (t : Technique) (n: network_map),
-      one_step a t n a' -> valid_attacker_i a'.
+Theorem one_step_preserves_valid_attacker_ii : forall (a a' : Attacker) (t : Technique) (n: network_map),
+      one_step a t n a' -> valid_attacker_ii a'.
   Proof.
     intros a a' t n onestep.
     destruct onestep.
     induction t; unfold valid_attacker in H0; unfold valid_concrete_network in H;
-    unfold Pre in H1; unfold Post in H2; unfold valid_attacker_i; intros m' u' known_machines_a'.
-    - apply (one_step_remote_services_preserves_valid_attacker_i a a' network H0 i i1 i0 i2 k i3); auto.
+    unfold Pre in H1; unfold Post in H2; unfold valid_attacker_ii.
     
   Admitted.
