Machine/MachineView.v
@@ -1,0 +1,40 @@
+Require Import Coq.Lists.List.
+Require Import Coq.Bool.Bool.
+Require Import Coq.Arith.EqNat.
+
+Require Import Machine.Machine.
+
+Section MachineView.
+
+  Definition subset_services (services1 services2: idService -> option Service) : Prop :=
+    forall (s: idService) (service: Service), services1 s = Some service -> services2 s = Some service.
+
+  Definition account_view (acc1 acc2: Account) : Prop :=
+    account_service acc1 = account_service acc2
+    /\ (account_key acc1 = None \/ account_key acc1 = account_key acc2)
+    /\ (account_privilege acc1 = None \/ account_privilege acc1 = account_privilege acc2).
+  
+  Definition sublist_accounts (l1 l2: list Account) : Prop :=
+    forall (acc: Account), In acc l1 -> (In acc l2 \/ (exists (acc': Account), In acc' l2 /\ account_view acc acc')).
+  
+  Definition subset_accounts (users1 users2: idUser -> option (list Account)) : Prop :=
+    forall (u: idUser) (l1 l2: list Account), users1 u = Some l1 -> users2 u = Some l2 -> sublist_accounts l1 l2.
+
+  Definition subset_files (files1 files2: path -> option (list path * list idUser * objective)) : Prop :=
+    True.
+
+  Definition subset_neighbours (l1 l2: list idMachine) : Prop :=
+    forall (m: idMachine), In m l1 -> In m l2.
+  
+  
+  Definition is_machineView (m1 m2: Machine) : Prop :=
+    subset_services (machine_services m1) (machine_services m2)
+    /\ subset_accounts (machine_accounts m1) (machine_accounts m2)
+    /\ subset_files (machine_fileSystem m1) (machine_fileSystem m2)
+    /\ subset_neighbours (machine_neighbours m1) (machine_neighbours m2).
+
+  Definition is_networkView (net1 net2: network_map) : Prop :=
+    forall (m: idMachine) (mac1 mac2: Machine), net1 m = Some mac1 -> net2 m = Some mac2 -> is_machineView mac1 mac2.
+
+
+End MachineView.
